module Associativity where

open import Data.Nat using (ℕ; zero; suc; _+_)
import Relation.Binary.PropositionalEquality as Eq
open Eq using (_≡_; cong)
open Eq.≡-Reasoning using (begin_; _≡⟨⟩_; _≡⟨_⟩_; _∎)

+-assoc : ∀ (m n p : ℕ) → (m + n) + p ≡ m + (n + p)
+-assoc zero n p =
  begin
    (zero + n) + p
  ≡⟨⟩
    n + p
  ≡⟨⟩
    zero + (n + p)
  ∎
+-assoc (suc m) n p =
  begin
    (suc m + n) + p
  ≡⟨⟩
    suc (m + n) + p
  ≡⟨⟩
    suc ((m + n) + p)
  ≡⟨ cong suc (+-assoc m n p) ⟩
    suc (m + (n + p))
  ≡⟨⟩
    suc m + (n + p)
  ∎
